Move taints into vale_heap_layout and have validSrcAddrs64 take a vale_heap_layout instead of just the taints.

vale/code/arch/Vale.Arch.Heap.fst
@@ -9,15 +9,14 @@ let heap_impl = vale_full_heap
 
 let heap_get hi = hi.vf_heap.mh
 
-let heap_taint hi = hi.vf_taint
+let heap_taint hi = hi.vf_layout.vl_taint
 
 let heap_upd hi mh' mt' =
   let h' = mi_heap_upd hi.vf_heap mh' in
   {
-    vf_layout = hi.vf_layout;
+    vf_layout = {hi.vf_layout with vl_taint = mt'};
     vf_heap = h';
     vf_heaplets = Map16.upd hi.vf_heaplets 0 h';
-    vf_taint = mt';
   }
 
 let heap_create_machine ih =
@@ -27,9 +26,12 @@ let heap_create_impl ih mt =
   let vh = ValeHeap (down_mem ih) (Ghost.hide ih) in
   let vh4 = ((vh, vh), (vh, vh)) in
   let vh16 = ((vh4, vh4), (vh4, vh4)) in
+  let layout_inner = {
+    vl_old_heap = vh;
+  } in
+  let layout = {vl_inner = layout_inner; vl_taint = mt;} in
   {
-    vf_layout = {vl_old_heap = vh};
+    vf_layout = layout;
     vf_heap = vh;
     vf_heaplets = Map16.upd vh16 0 vh;
-    vf_taint = mt;
   }
