vale/code/arch/Vale.Arch.HeapImpl.fsti
@@ -15,12 +15,18 @@ This splitting is done to avoid circular module dependencies.
 let heaplet_id = n:nat{n < 16}
 
 val vale_heap : Type u#1
-val vale_heap_layout : Type u#1
+val vale_heap_layout_inner : Type u#1
+
+noeq type vale_heap_layout : Type u#1 = {
+  vl_inner:vale_heap_layout_inner;
+  vl_taint:memTaint_t;
+}
 
 noeq type vale_full_heap = {
   vf_layout:vale_heap_layout;
   vf_heap:vale_heap;
   vf_heaplets:Vale.Lib.Map16.map16 vale_heap;
-  vf_taint:memTaint_t;
 }
 
+unfold let full_heap_taint (vfh:vale_full_heap) : memTaint_t =
+  vfh.vf_layout.vl_taint
