vale/code/arch/x64/Vale.X64.InsLemmas.fst
@@ -32,11 +32,11 @@ let lemma_valid_src_operand64_and_taint o s =
   | OMem (m, t) ->
     let addr = eval_maddr m s in
     let aux (b:buffer64) (i:int) : Lemma
-      (requires valid_buf_maddr64 addr h s.vs_heap.vf_taint b i t)
+      (requires valid_buf_maddr64 addr h s.vs_heap.vf_layout b i t)
       (ensures S.valid_src_operand64_and_taint o (state_to_S s))
       =
       lemma_heap_get_heap s.vs_heap;
-      lemma_valid_taint64 b s.vs_heap.vf_taint h i t
+      lemma_valid_taint64 b (full_heap_taint s.vs_heap) h i t
       in
     Classical.forall_intro_2 (fun b i -> (fun b -> Classical.move_requires (aux b)) b i)
   | OStack (m, t) -> lemma_valid_taint_stack64 (eval_maddr m s) t s.vs_stackTaint
@@ -48,11 +48,11 @@ let lemma_valid_src_operand128_and_taint o s =
   | OMem (m, t) ->
     let addr = eval_maddr m s in
     let aux (b:buffer128) (i:int) : Lemma
-      (requires valid_buf_maddr128 addr h s.vs_heap.vf_taint b i t)
+      (requires valid_buf_maddr128 addr h s.vs_heap.vf_layout b i t)
       (ensures S.valid_src_operand128_and_taint o (state_to_S s))
       =
       lemma_heap_get_heap s.vs_heap;
-      lemma_valid_taint128 b s.vs_heap.vf_taint h i t
+      lemma_valid_taint128 b (full_heap_taint s.vs_heap) h i t
       in
     Classical.forall_intro_2 (fun b i -> (fun b -> Classical.move_requires (aux b)) b i)
   | OStack (m, t) -> lemma_valid_taint_stack128 (eval_maddr m s) t s.vs_stackTaint
